src/QFBVSimple.v
@@ -91,7 +91,7 @@ Module Make (V : SsrOrderedType) (A : Arch).
     | bvLshr w e1 e2 => fromNat 0 (* TODO *)
     | bvAshr w e1 e2 => fromNat 0 (* TODO *)
     | bvConcat w1 w2 e1 e2 => catB (eval_exp e1 s) (eval_exp e2 s)
-    | bvExtract w i j e => fromNat 0 (* TODO *)
+    | bvExtract w i j e => slice j (i-j+1) w (eval_exp e s)
     | bvSlice w1 w2 w3 e => slice w3 w2 w1 (eval_exp e s)
     | bvHigh wh wl e => high wh (eval_exp e s)
     | bvLow wh wl e => low wl (eval_exp e s)
